\documentclass[aps,pre,nofootinbib]{revtex4}

\usepackage{amsmath,amssymb,amsfonts,amsthm}
\usepackage{graphicx}
\usepackage{bbm}
\usepackage{pdfsync}
\usepackage{color}

\begin{document}

\title{Problem Set XXXI}

\author{Gray Davidson}
\affiliation{Department of Physics, Reed College, Portland, Oregon,  97202, USA}
\date{\today}
\maketitle

\section{31.0}
For your grading pleasure, we (Gray Davidson) has on this occasion decided to begin tex-ing his homework.  We'll see how this goes.  

\section{31.1}
Griffiths 5.1

\bigskip
Given vectors $\vec{r_1}$ and $\vec{r_2}$ we define: 

\begin{equation}
\vec{r} = \vec{r_1}-\vec{r_2}
\end{equation}

and 

\begin{equation}
\vec{R} = \frac{m_1 \vec{r_1} + m_2 \vec{r_2}}{m_1 + m_2}
\end{equation}

a)
\begin{equation}
\vec{r_1} = \vec{R}+\frac{\mu}{m_1} \vec{r}
\end{equation}

\begin{equation}
\vec{r_1} =\frac{m_1 \vec{r_1} + m_2 \vec{r_2}}{m_1 + m_2}+\frac{\mu}{m_1}(\vec{r_1}-\vec{r_2})
\end{equation}

\begin{equation}
\vec{r_1} =\frac{m_1 \vec{r_1} + m_2 \vec{r_2} + m_2 \vec{r_1} - m_2\vec{r_2}}{m_1 + m_2}
\end{equation}

\begin{equation}
\vec{r_1} =\frac{m_1 + m_2}{m_1 + m_2}\vec{r_1}
\end{equation}

\begin{equation}
\vec{r_1} =\vec{r_1}
\end{equation}

And likewise for $\vec{r_2}$

\begin{equation}
\vec{r_2} = \vec{R}-\frac{\mu}{m_2} \vec{r}
\end{equation}

\begin{equation}
\vec{r_2} =\frac{m_1 \vec{r_1} + m_2 \vec{r_2}}{m_1 + m_2}-\frac{\mu}{m_2}(\vec{r_1}-\vec{r_2})
\end{equation}

\begin{equation}
\vec{r_2} =\frac{m_1 \vec{r_1} + m_2 \vec{r_2} - m_1 \vec{r_1} + m_1\vec{r_2}}{m_1 + m_2}
\end{equation}

\begin{equation}
\vec{r_2} =\frac{m_1 + m_2}{m_1 + m_2}\vec{r_2}
\end{equation}

\begin{equation}
\vec{r_2} =\vec{r_2}
\end{equation}

We attempt to make some sense of the derivatives, but find that something in our definition is wrong.  We are using the following equations: 
 
\begin{equation}
\nabla_r  = \nabla_1 - \nabla_2
\end{equation}

and

\begin{equation}
\nabla_R = \frac{m_1 \nabla_1 + m_2 \nabla_2}{m_1 + m_2}
\end{equation}

\begin{equation}
\nabla_1 = \frac{\mu}{m2}\frac{m_1 \nabla_1 + m_2 \nabla_2}{m_1 + m_2} + \nabla_1 - \nabla_2
\end{equation}

\begin{equation}
\nabla_1 = \frac{\mu}{m2}\nabla_R + \nabla_r
\end{equation}

and also:

\begin{equation}
\nabla_2 = \frac{\mu}{m_1}\frac{m_1 \nabla_1 + m_2 \nabla_2}{m_1 + m_2} - \nabla_1 + \nabla_2
\end{equation}

\begin{equation}
\nabla_2 = \frac{\mu}{m2}\nabla_R - \nabla_r
\end{equation}

Man, this is not as easy as it sounds.  I'll try again in future, but for now, I must go back to handwritten work.
\end{document}
